deps/k-x86-semantics/k-semantics/popw.lean
@@ -1,0 +1,11 @@
+def popw : instruction :=
+  definst "popw" $ do
+    instr_pat $ fun (mem_0 : Mem) =>
+     let action : semantics Unit := do
+      let v_1 <- getRegister rsp;
+      setRegister rsp (add v_1 (expression.bv_nat 64 2));
+      let v_3 <- evaluateAddress mem_0;
+      let v_4 <- load v_1 2;
+      store v_3 v_4 2;
+      pure ()
+     action
